theories/CertiGC/vst/proof/verif_create_heap.v
@@ -18,7 +18,7 @@ Proof.
 Qed.
 
 Lemma split2_data_at_Tarray_space_type:
-  forall (sh: share) (n n1: Z) (v: list (val * (val * val))) (p: val),
+  forall (sh: share) (n n1: Z) (v: list (reptype space_type)) (p: val),
     0 <= n1 <= n -> n = Zlength v ->
     data_at sh (tarray space_type n) v p =
     data_at sh (tarray space_type n1) (sublist 0 n1 v) p *
@@ -31,7 +31,7 @@ Proof.
   - rewrite sublist_all; [|apply Z.eq_le_incl; rewrite H0]; reflexivity.
 Qed.
 
-Lemma space_array_1_eq: forall (sh: share) (v: (val * (val * val))) (p: val),
+Lemma space_array_1_eq: forall (sh: share) (v: reptype space_type) (p: val),
     data_at sh (tarray space_type 1) [v] p = data_at sh space_type v p.
 Proof.
   intros. pose proof (data_at_singleton_array_eq sh space_type). apply H. reflexivity.
@@ -81,11 +81,11 @@ Proof.
       exfalso; assumption.
   - Intros. forward_if True; [contradiction | forward; entailer! |]. Intros.
     (* make "data_at sh space_type v h " in SEP *)
-    assert_PROP (isptr h) by entailer!. remember (Vundef, (Vundef, Vundef)) as vn.
+    assert_PROP (isptr h) by entailer!. remember (Vundef, (Vundef, (Vundef, Vundef))) as vn.
     assert_PROP (field_compatible heap_type [StructField _spaces] h) by entailer!.
     replace_SEP 2 (data_at Ews heap_type (default_val heap_type) h) by entailer!.
     change (default_val heap_type) with
-        (repeat (Vundef, (Vundef, Vundef)) (Z.to_nat 12)).
+        (repeat (Vundef, (Vundef, (Vundef, Vundef))) (Z.to_nat 12)).
     rewrite <- Heqvn. rewrite data_at_heaptype_eq; auto.
     rewrite (split2_data_at_Tarray_space_type Ews 12 1);
       [| lia | rewrite Zlength_repeat; lia].
@@ -99,20 +99,31 @@ Proof.
       change (12 - 1) with 11 at 2.
       gather_SEP (data_at Ews (tarray space_type 1) _ h)
                  (data_at Ews (tarray space_type (12 - 1)) _ _).
-      remember (p0, (p0, offset_val (WORD_SIZE * Z.shiftl 1 16) p0)) as vh.
+      remember (p0, (p0, (offset_val (WORD_SIZE * Z.shiftl 1 16) p0, offset_val (WORD_SIZE * Z.shiftl 1 16) p0))) as vh.
       remember (vh :: repeat vn (Z.to_nat 11)) as vl.
       replace [vh] with (sublist 0 1 vl). 2: {
         subst vl; rewrite sublist_one; try lia.
         - rewrite Znth_0_cons; auto.
         - rewrite Zlength_cons, Zlength_repeat; lia.
-      } replace (repeat  vn (Z.to_nat 11)) with (sublist 1 12 vl) by
+      }
+      replace (repeat  vn (Z.to_nat 11)) with (sublist 1 12 vl) by
           (rewrite Heqvl, sublist_1_cons, sublist_repeat; [reflexivity|lia..]).
-      rewrite <- split2_data_at_Tarray_space_type;
-        [| lia | rewrite Heqvl, Zlength_cons, Zlength_repeat; lia].
-      remember (if Archi.ptr64 then
-                  (Vlong (Int64.repr 0),
-                   (Vlong (Int64.repr 0), Vlong (Int64.repr 0))) else
-                  (Vint (Int.repr 0), (Vint (Int.repr 0), Vint (Int.repr 0)))) as v0.
+      rewrite <- (split2_data_at_Tarray_space_type Ews 12 1 (vh :: repeat vn (Z.to_nat 11))) ; try lia ; try easy.
+      remember (
+        if Archi.ptr64
+        then
+          ( Vlong (Int64.repr 0),
+          ( Vlong (Int64.repr 0),
+          ( Vlong (Int64.repr 0)
+          , Vlong (Int64.repr 0)
+          )))
+        else
+          ( Vint (Int.repr 0),
+          ( Vint (Int.repr 0),
+          ( Vint (Int.repr 0)
+          , Vint (Int.repr 0)
+          )))
+      ) as v0.
       (* change succeed *) subst vl. rewrite <- data_at_heaptype_eq; auto.
       cbv [Archi.ptr64] in Heqv0.
       forward_for_simple_bound
@@ -120,32 +131,47 @@ Proof.
         (EX i: Z,
          PROP ( )
          LOCAL (temp _h h; gvars gv)
-         SEP (data_at Ews heap_type
-                      (vh :: repeat v0 (Z.to_nat (i - 1)) ++
-                          repeat vn (Z.to_nat (12 - i))) h; FRZL FR))%assert.
+         SEP (data_at
+                Ews heap_type
+                (vh :: repeat v0 (Z.to_nat (i - 1)) ++ repeat vn (Z.to_nat (12 - i)))
+                h;
+                FRZL FR
+              )
+        )%assert.
       * entailer!.
-      * Opaque Znth. forward. rewrite (repeat_cons (12 - i)) at 2 by lia.
+      * Opaque Znth.
+        forward.
+        rewrite (repeat_cons (12 - i)) at 2 by lia.
         rewrite Znth_repeat_app by apply (proj1 H2). rewrite Heqvn at 2.
         rewrite (repeat_cons (12 - i)) by lia.
-        rewrite upd_Znth_repeat_app by apply (proj1 H2). forward.
+        rewrite upd_Znth_repeat_app by apply (proj1 H2).
+        forward.
         rewrite Znth_repeat_app by apply (proj1 H2).
-        rewrite upd_Znth_repeat_app by apply (proj1 H2). forward.
+        rewrite upd_Znth_repeat_app by apply (proj1 H2).
+        forward.
+        rewrite Znth_repeat_app by apply (proj1 H2).
+        rewrite upd_Znth_repeat_app by apply (proj1 H2).
+        forward.
         rewrite Znth_repeat_app by apply (proj1 H2).
         rewrite upd_Znth_repeat_app by apply (proj1 H2).
         simpl fst.
-        replace (i + 1 - 1) with i by lia. try rewrite !Int.signed_repr by rep_lia.
-        rewrite <- Heqv0. replace (12 - i - 1) with (12 - (i + 1)) by lia.
+        replace (i + 1 - 1) with i by lia.
+        try rewrite !Int.signed_repr by rep_lia.
+        rewrite <- Heqv0.
+        replace (12 - i - 1) with (12 - (i + 1)) by lia.
         change (v0 :: repeat vn (Z.to_nat (12 - (i + 1))))
                with ([v0] ++ repeat vn (Z.to_nat (12 - (i + 1)))).
         rewrite app_assoc.
-        replace (repeat v0 (Z.to_nat (i - 1)) ++ [v0]) with
-            (repeat v0 (Z.to_nat i)). 1: entailer!.
-        replace [v0] with (repeat v0 (Z.to_nat 1)) by (simpl; auto).
-        rewrite <- repeat_app. f_equal. rewrite <- Z2Nat.inj_add by lia.
-        f_equal. lia.
+        replace (repeat v0 (Z.to_nat (i - 1)) ++ [v0]) with (repeat v0 (Z.to_nat i)).
+        2: {
+          replace [v0] with (repeat v0 (Z.to_nat 1)) by (simpl; auto).
+          rewrite <- repeat_app. f_equal. rewrite <- Z2Nat.inj_add by lia.
+          f_equal. lia.
+        }
+        entailer!.
       * replace (12 - 12) with 0 by lia. simpl repeat at 2.
         rewrite app_nil_r. change 12 with MAX_SPACES at 2. thaw FR.
         change (Z.shiftl 1 16) with NURSERY_SIZE in *.
-        assert (v0 = zero_triple) by (subst v0; unfold zero_triple; reflexivity).
+        assert (v0 = nullspace) by (subst v0; unfold nullspace; reflexivity).
         rewrite H2. forward. Exists h p0. entailer!. Transparent Znth.
 Qed.
