theories/CertiGC/vst/proof/verif_do_scan.v
@@ -87,7 +87,7 @@ Proof.
     remember (Znth (Z.of_nat to) (heap_spaces (ti_heap t_info'))) as sp_to.
     assert (isptr (space_base sp_to)) by (rewrite <- H18; apply generation_base__isptr).
     remember (map space_tri (heap_spaces (ti_heap t_info'))).
-    assert (@Znth (val * (val * val)) (Vundef, (Vundef, Vundef))
+    assert (@Znth (val * (val * (val * val))) (Vundef, (Vundef, (Vundef, Vundef)))
                   (Z.of_nat to) l = space_tri sp_to). {
       subst l sp_to. now rewrite Znth_map by (rewrite heap_spaces__size; rep_lia). }
     forward; rewrite H22; unfold space_tri. 1: entailer!.
